src/ppprover.ml
@@ -110,6 +110,17 @@ let output_state o st =
   Printf.fprintf o "Units : %a\n" (output_units st.hconsmap) st.units;
   Printf.fprintf o "Clauses : %a\n" output_clauses st.clauses
 
+
+
+let output_plit o hm p =
+  PLit.fold (fun () k b ->
+      match IntMap.get' kInt k hm with
+      | None -> failwith "Unknow literal"
+      | Some (b',f) ->
+         match b with
+         | None   -> Printf.fprintf o "Err : %a" output_bformula f
+         | Some b -> Printf.fprintf o "Err : %b %a" b  output_bformula  f) p ()
+             
 (**  *)
 
 (** *)
